theories/language/progenv.v
@@ -6,7 +6,7 @@ From iris.prelude Require Import options.
 
 Record prog_environ `{!indexT} {val} (Λ : language val) Σ := Penv {
   penv_prog : gmap string Λ.(func);
-  penv_proto : string -d> list val -d> (val -d> iPropO Σ) -d> iPropO Σ;
+  penv_proto : string -d> list val -d> ((outcome val) -d> iPropO Σ) -d> iPropO Σ;
 }.
 Global Arguments Penv {_ _ _ _} _ _.
 Global Arguments penv_prog {_ _ _ _} _.
